Small improvement.

Extensions/ShallowEmbedded/MonoPredicateStable.v
@@ -22,13 +22,15 @@ Require Import Logic.PropositionalLogic.ShallowEmbedded.MonoPredicateProposition
 Require Import Logic.ModalLogic.ShallowEmbedded.MonoPredicateModalLogic.
 Require Import Logic.SeparationLogic.ShallowEmbedded.MonoPredicateSeparationLogic.
 
+Definition MonoPred_stable (A: Type) {R1: KI.Relation A} {kiM: KripkeIntuitionisticModel A} {R2: SS.Relation A}: expr -> Prop := fun x => Semantics.stable (@Kdenotation _ (Build_Model A) (unit_kMD _) tt _ x).
+
 Instance MonoPred_stableSM (A: Type) {R1: KI.Relation A} {kiM: KripkeIntuitionisticModel A} {R2: SS.Relation A}: @SemanticStable (MonoPred_L A) (Build_Model A) (unit_kMD _) tt R2 (MonoPred_SM A).
 Proof.
-  refine (Build_SemanticStable _ _ _ _ _ _ (fun x => Semantics.stable (@Kdenotation _ _ (unit_kMD _) tt _ x)) _).
+  refine (Build_SemanticStable _ _ _ _ _ _ (MonoPred_stable A) _).
   intros. reflexivity.
 Defined.
 
-Instance MonoPred_pstable (A: Type) {R1: KI.Relation A} {kiM: KripkeIntuitionisticModel A} {R2: SS.Relation A} {KI_bis_R2: KripkeIntuitionisticBisStable A}: PropositionalStable (MonoPred_L A) (MonoPred_Gamma A) (fun x => Semantics.stable (@Kdenotation _ (Build_Model A) (unit_kMD _) tt _ x)).
+Instance MonoPred_pstable (A: Type) {R1: KI.Relation A} {kiM: KripkeIntuitionisticModel A} {R2: SS.Relation A} {KI_bis_R2: KripkeIntuitionisticBisStable A}: PropositionalStable (MonoPred_L A) (MonoPred_Gamma A) (MonoPred_stable A).
 Proof.
   constructor.
   + intros x y.
@@ -42,21 +44,21 @@ Proof.
     exact (@Sound_KripkeIntuitionistic.sound_stable_proper_iffp (MonoPred_L A) _ _ (Build_Model A) (unit_kMD _) tt R1 _ _ (MonoPred_SM A) (MonoPred_kiSM A) (MonoPred_stableSM A) x y).
 Qed.
 
-Instance MonoPred_mstable (A: Type) {R1: KI.Relation A} {kiM: KripkeIntuitionisticModel A} {R2: KM.Relation A} {R3: SS.Relation A} {ukmM: UpwardsClosedOrderedKripkeModel A} {KM_bis_R3: KripkeModalBisStable A}: ModalStable (MonoPred_L A) (MonoPred_Gamma A) (fun x => Semantics.stable (@Kdenotation _ (Build_Model A) (unit_kMD _) tt _ x)).
+Instance MonoPred_mstable (A: Type) {R1: KI.Relation A} {kiM: KripkeIntuitionisticModel A} {R2: KM.Relation A} {R3: SS.Relation A} {ukmM: UpwardsClosedOrderedKripkeModel A} {KM_bis_R3: KripkeModalBisStable A}: ModalStable (MonoPred_L A) (MonoPred_Gamma A) (MonoPred_stable A).
 Proof.
   constructor.
   intros x.
   exact (@Sound_KripkeIntuitionistic.sound_boxp_stable (MonoPred_L A) _ _ _ (Build_Model A) (unit_kMD _) tt R1 _ _ _ (MonoPred_SM A) (MonoPred_fmSM A) (MonoPred_stableSM A) x).
 Qed.
 
-Instance MonoPred_MAS (A: Type) {R1: KI.Relation A} {kiM: KripkeIntuitionisticModel A} {R2: KM.Relation A} {R3: SS.Relation A} {ukmM: UpwardsClosedOrderedKripkeModel A} {KM_abs_R3: KripkeModalAbsorbStable A}: ModalAbsorbStable (MonoPred_L A) (MonoPred_Gamma A) (fun x => Semantics.stable (@Kdenotation _ (Build_Model A) (unit_kMD _) tt _ x)).
+Instance MonoPred_MAS (A: Type) {R1: KI.Relation A} {kiM: KripkeIntuitionisticModel A} {R2: KM.Relation A} {R3: SS.Relation A} {ukmM: UpwardsClosedOrderedKripkeModel A} {KM_abs_R3: KripkeModalAbsorbStable A}: ModalAbsorbStable (MonoPred_L A) (MonoPred_Gamma A) (MonoPred_stable A).
 Proof.
   constructor.
   intros x.
   exact (@Sound_KripkeIntuitionistic.sound_boxp_absorb_stable (MonoPred_L A) _ _ _ (Build_Model A) (unit_kMD _) tt R1 _ _ _ (MonoPred_SM A) (MonoPred_kiSM A) (MonoPred_fmSM A) (MonoPred_stableSM A) x).
 Qed.
 
-Instance MonoPred_sstable (A: Type) {R1: KI.Relation A} {kiM: KripkeIntuitionisticModel A} {J: Join A} {SA: SeparationAlgebra A} {uSA: UpwardsClosedSeparationAlgebra A} {dSA: DownwardsClosedSeparationAlgebra A} {R2: SS.Relation A} {SA_bis_R2: SeparationAlgebraBisStable A}: SeparationStable (MonoPred_L A) (MonoPred_Gamma A) (fun x => Semantics.stable (@Kdenotation _ (Build_Model A) (unit_kMD _) tt _ x)).
+Instance MonoPred_sstable (A: Type) {R1: KI.Relation A} {kiM: KripkeIntuitionisticModel A} {J: Join A} {SA: SeparationAlgebra A} {uSA: UpwardsClosedSeparationAlgebra A} {dSA: DownwardsClosedSeparationAlgebra A} {R2: SS.Relation A} {SA_bis_R2: SeparationAlgebraBisStable A}: SeparationStable (MonoPred_L A) (MonoPred_Gamma A) (MonoPred_stable A).
 Proof.
   constructor.
   + intros x y.
@@ -65,7 +67,7 @@ Proof.
     exact (@Sound_KripkeIntuitionistic.sound_wand_stable (MonoPred_L A) _ _ _ (Build_Model A) (unit_kMD _) tt R1 _ _ _ (MonoPred_SM A) (MonoPred_fsSM A) (MonoPred_stableSM A) x y).
 Qed.
 
-Instance MonoPred_SAS (A: Type) {R1: KI.Relation A} {kiM: KripkeIntuitionisticModel A} {J: Join A} {SA: SeparationAlgebra A} {uSA: UpwardsClosedSeparationAlgebra A} {dSA: DownwardsClosedSeparationAlgebra A} {R2: SS.Relation A} {SA_abs_R2: SeparationAlgebraAbsorbStable A}: SeparationAbsorbStable (MonoPred_L A) (MonoPred_Gamma A) (fun x => Semantics.stable (@Kdenotation _ (Build_Model A) (unit_kMD _) tt _ x)).
+Instance MonoPred_SAS (A: Type) {R1: KI.Relation A} {kiM: KripkeIntuitionisticModel A} {J: Join A} {SA: SeparationAlgebra A} {uSA: UpwardsClosedSeparationAlgebra A} {dSA: DownwardsClosedSeparationAlgebra A} {R2: SS.Relation A} {SA_abs_R2: SeparationAlgebraAbsorbStable A}: SeparationAbsorbStable (MonoPred_L A) (MonoPred_Gamma A) (MonoPred_stable A).
 Proof.
   constructor.
   intros x y z.
